Bignum/ComponentExtra.lean
@@ -1,0 +1,21 @@
+/-
+Copyright (c) 2026 Guilherme Lima. All rights reserved.
+Released under Apache 2.0 license as described in the file LICENSE.
+Author: Guilherme Lima
+-/
+module
+
+public import Bignum.BitVec
+public import Bignum.Component
+
+@[expose] public section
+
+set_option autoImplicit false
+
+namespace Bignum.Component
+
+/-- Component for a bit within a BitVec. -/
+def bitelement {w : Nat} (i : Fin w) : Component (BitVec w) Bool :=
+  ⟨λ bv ↦ bv.getLsb i, λ b bv ↦ BitVec.setLsb bv i b⟩
+
+end Bignum.Component
