BignumTest/ComponentExtra.lean
@@ -1,0 +1,19 @@
+/-
+Copyright (c) 2026 Guilherme Lima. All rights reserved.
+Released under Apache 2.0 license as described in the file LICENSE.
+Author: Guilherme Lima
+-/
+
+import Bignum.ComponentExtra
+
+open Bignum
+
+section bitelement
+def bv : BitVec 8 := 0b01001011#8
+example : (Component.bitelement 0).read bv = true := by rfl
+example : (Component.bitelement 1).read bv = true := by rfl
+example : (Component.bitelement 2).read bv = false := by rfl
+example : (Component.bitelement 3).read bv = true := by rfl
+def bv' := (Component.bitelement 3).write false bv
+example : bv' = 0b01000011#8 := by rfl
+end bitelement
